fixed realaxTheory issue

semantics/chorTypeScript.sml
@@ -7,26 +7,27 @@ val _ = new_theory "chorType";
 
 Inductive chorTypecheckOK:
 [~nil:] ∀ Γ Θ. chorTypecheckOK Γ Θ Nil
-[~com:] ∀ Γ Θ p1 v1 p2 v2 c ty. FLOOKUP Γ (v1,p1) = SOME strT ∧
-                                FLOOKUP Γ (v2,p2) = SOME strT ∧
-                                ({p1;p2} ⊆ Θ) ∧
-                                chorTypecheckOK Γ Θ c ⇒
-                                chorTypecheckOK Γ Θ (Com p1 v1 p2 v2 c)
-[~sel:] ∀ Γ Θ p1 p2 b c ty. ({p1;p2} ⊆ Θ) ∧ chorTypecheckOK Γ Θ c ⇒
-                            chorTypecheckOK Γ Θ (Sel p1 b p2 c)
-[~if:] ∀ Γ Θ v p c1 c2 ty. FLOOKUP Γ (v,p) = SOME boolT ∧
-                           chorTypecheckOK Γ Θ c1 ∧ chorTypecheckOK Γ Θ c2 ⇒
-                           chorTypecheckOK Γ Θ (IfThen v p c1 c2)
+[~com:] ∀ Γ Θ p1 v1 p2 v2 c. FLOOKUP Γ (v1,p1) = SOME strT ∧
+                             FLOOKUP Γ (v2,p2) = SOME strT ∧
+                             ({p1;p2} ⊆ Θ) ∧
+                             chorTypecheckOK Γ Θ c ⇒
+                             chorTypecheckOK Γ Θ (Com p1 v1 p2 v2 c)
+[~sel:] ∀ Γ Θ p1 p2 b c. ({p1;p2} ⊆ Θ) ∧ chorTypecheckOK Γ Θ c ⇒
+                         chorTypecheckOK Γ Θ (Sel p1 b p2 c)
+[~if:] ∀ Γ Θ v p c1 c2. FLOOKUP Γ (v,p) = SOME boolT ∧
+                        chorTypecheckOK Γ Θ c1 ∧ chorTypecheckOK Γ Θ c2 ⇒
+                        chorTypecheckOK Γ Θ (IfThen v p c1 c2)
 [~let:] ∀ Γ Θ v p e c ety. typecheck (localise Γ p) e ety ∧
                            chorTypecheckOK (Γ |+ ((v,p), ety)) Θ c ⇒
                            chorTypecheckOK Γ Θ (Let v p e c)
-[~fix:] ∀ Γ Θ c. chorTypecheckOK Γ (Θ ∪ {dn}) c ⇒ chorTypecheckOK Γ Θ (Fix dn c)
+[~fix:] ∀ Γ Θ c dn. chorTypecheckOK Γ (Θ ∪ {dn}) c ⇒ chorTypecheckOK Γ Θ (Fix dn c)
+[~call:] ∀ Γ Θ dn. {dn} ⊆ Θ ⇒ chorTypecheckOK Γ Θ (Call dn)
 End
 
 Definition chorEnvtype_def:
-  chorEnvtype Γ Δ = ∀ str p ty. FLOOKUP Γ (str,p) = SOME ty ⇒
-                                ∃ v. FLOOKUP Δ (str,p) = SOME v ∧ value_type v ty
+  chorEnvtype Γ Δ = (∀ p. envtype (localise Γ p) (localise Δ p))
 End
 
+        
 val _ = export_theory();
 
