semantics/proofs/chorTypePropsScript.sml
@@ -1,0 +1,62 @@
+open HolKernel Parse boolLib bossLib chorSemTheory chorLangTheory richerLangTheory valueTheory envSemTheory chorPropsTheory chorTypeTheory finite_mapTheory pred_setTheory
+
+val _ = new_theory "chorTypeProps";
+
+Theorem chortype_localise_fdom:
+  ∀ p. chorEnvtype Γ Δ ⇒ FDOM (localise Γ p) ⊆ FDOM (localise Δ p)
+Proof
+  rw[chorEnvtype_def, envtype_fdom]
+QED
+
+Theorem chortype_fdom_subset:
+  chorEnvtype Γ Δ ⇒ FDOM Γ ⊆ FDOM Δ
+Proof
+  rw[chortype_localise_fdom, localise_fdom_subset]
+QED
+
+Theorem chortype_update:
+  chorEnvtype Γ Δ ∧ value_type v ty ⇒
+  ∀ vn p. chorEnvtype (Γ |+ ((vn,p), ty)) (Δ |+ ((vn,p), v))
+Proof
+  rw[chorEnvtype_def] >>
+  ‘envtype (localise Γ p' |+ (vn, ty)) (localise Δ p' |+ (vn, v))’ by metis_tac[envtype_update] >> Cases_on ‘p' = p’
+  >- gvs[localise_update_eqn]
+  >> metis_tac[localise_update_neq]
+QED
+
+Theorem type_has_exp:
+  ∀ G ty. ∃ e. typecheck G e ty
+Proof
+  Induct_on ‘ty’ >> rw[] >~
+  [‘pairT t1 t2’]
+  >- (irule_at Any typecheck_Binop >> metis_tac[boptype_rules])
+  >> metis_tac[typecheck_rules, uoptype_rules]
+QED
+
+Theorem type_has_value:
+  ∀ ty. ∃ v. value_type v ty
+Proof
+  Induct >~
+  [‘fnT aty bty’]
+  >- (irule_at Any value_type_FnV >>
+      ‘∃ e. typecheck (FEMPTY |+ (s,aty)) e bty’ by metis_tac[type_has_exp] >>
+      first_assum $ irule_at Any >> simp[])
+  >> metis_tac[value_type_rules]
+QED
+
+Theorem chortype_no_undefined_vars:
+  ∀ Γ Θ Δ. chorTypecheckOK Γ Θ c ∧ chorEnvtype Γ Δ ⇒
+  no_undefined_vars (Δ, c)
+Proof
+  Induct_on ‘chorTypecheckOK’ >> rw[no_undefined_vars_def, free_variables_def, Once chorTypecheckOK_cases, FLOOKUP_DEF]
+  >- metis_tac[chortype_fdom_subset, SUBSET_DEF]
+  >- ASM_SET_TAC []
+  >- metis_tac[chortype_fdom_subset, SUBSET_DEF]
+  >- metis_tac[typecheck_no_undefined_vars, subset_fdom_localise_state, chortype_localise_fdom, SUBSET_TRANS]
+  >> (‘∃ val. value_type val ety’ by simp[type_has_value] >>
+      drule_all chortype_update >> disch_then $ qspecl_then [‘v’, ‘p’] assume_tac >>
+      first_x_assum drule >> simp[] >> SET_TAC [])
+QED
+
+val _ = export_theory();
+
